NLustreToSyBloc/Translation.v
@@ -706,6 +706,10 @@ Module Type TRANSLATION
        SynSB.b_out  := idty n.(n_out);
        SynSB.b_eqs  := translate_eqns n.(n_eqs)
     |}.
+  Next Obligation.
+    destruct n; simpl.
+    now rewrite length_idty.
+  Qed.
   (* (* =end= *) *)
   (* Next Obligation. *)
   (*   repeat rewrite <-idty_app. rewrite NoDupMembers_idty. *)
